Basic intrinsic term typing

Isotope/Syntax/Intrinsic/Basic.lean
@@ -31,6 +31,10 @@ structure Transparency where
 def HasLin.lin {T} [HasLin T] (t: T) (l: Transparency): Bool
   := (l.aff → HasLin.aff t) ∧ (l.rel → HasLin.rel t)
 
+instance Transparency.instHasLin: HasLin Transparency where
+  aff := Transparency.aff
+  rel := Transparency.rel
+
 instance Transparency.instPartialOrder: PartialOrder Transparency where
   le l r := l.aff ≤ r.aff ∧ l.rel ≤ r.rel
   le_refl := by simp
@@ -45,30 +49,44 @@ theorem Transparency.le.rel {l r: Transparency}
   : l ≤ r → l.rel → r.rel := And.right
 
 --TODO: add resource algebra to variables?
-structure Variable (T: Type u) extends Transparency where
+structure Var (T: Type u) extends Transparency where
   ty: Ty T
 
-instance Variable.instHasLin {T} [HasLin T]: HasLin (Variable T) where
+instance Var.instHasLin {T} [HasLin T]: HasLin (Var T) where
   aff v := v.aff && HasLin.aff v.ty
   rel v := v.rel && HasLin.rel v.ty
 
-instance Variable.instPartialOrder {T}: PartialOrder (Variable T) where
+instance Var.instPartialOrder {T}: PartialOrder (Var T) where
   le l r := l.ty = r.ty ∧ l.toTransparency ≤ r.toTransparency
   le_refl := by simp [le_refl]
   le_trans _ _ _  | ⟨He, Ht⟩, ⟨He', Ht'⟩ => ⟨He.trans He', le_trans Ht Ht'⟩
   le_antisymm x x' H H'
     := mk.injEq _ _ _ _ ▸ ⟨le_antisymm H.2 H'.2, H.1⟩
 
-theorem Variable.le.aff {T} [HasLin T] {l r: Variable T}
+theorem Var.le.aff {T} [HasLin T] {l r: Var T}
   : l ≤ r → HasLin.aff l → HasLin.aff r
   | ⟨He, Ht⟩ => by
     simp only [HasLin.aff, He, Bool.and_eq_true, and_imp]
     intro H H';
     exact ⟨Ht.1 H, H'⟩
 
-theorem Variable.le.rel {T} [HasLin T] {l r: Variable T}
+theorem Var.le.rel {T} [HasLin T] {l r: Var T}
   : l ≤ r → HasLin.rel l → HasLin.rel r
   | ⟨He, Ht⟩ => by
     simp only [HasLin.rel, He, Bool.and_eq_true, and_imp]
     intro H H';
     exact ⟨Ht.2 H, H'⟩
+
+structure Comp (T: Type u) extends Var T where
+  cen: Bool
+
+instance Comp.instHasLin {T} [HasLin T]: HasLin (Var T) where
+  aff v := v.aff && HasLin.aff v.ty
+  rel v := v.rel && HasLin.rel v.ty
+
+instance Comp.instPartialOrder {T}: PartialOrder (Comp T) where
+  le l r := l.toVar ≤ r.toVar ∧ l.cen ≤ r.cen
+  le_refl := by simp [le_refl]
+  le_trans _ _ _  | ⟨He, Ht⟩, ⟨He', Ht'⟩ => ⟨le_trans He He', le_trans Ht Ht'⟩
+  le_antisymm x x' H H'
+    := mk.injEq _ _ _ _ ▸ ⟨le_antisymm H.1 H'.1, le_antisymm H.2 H'.2⟩
