Isotope/Syntax/Intrinsic.lean
@@ -1,14 +1,62 @@
-import Isotope.Syntax.Intrinsic.Ctx
+import Isotope.Syntax.Intrinsic.LCtx
 
-inductive Term {T} [HasLin T]: Ctx T -> Variable T -> Type
-  | var {Γ x} (v: Ctx.var Γ x): Term Γ x
+inductive GCtx (T: Type u) [HasLin T]: Type u
+  | df (Γ: Ctx T)
+  | cf (L: LCtx T)
+
+inductive Result (T: Type u) [HasLin T]: Type u
+  | term (x: Var T)
+  | label (L: LCtx T)
+
+class InstructionSet (F: Type u) (T: Type v)
+  where
+  inst_ty: F -> Ty T -> Ty T -> Prop
+  inst_aff: F -> Ty T -> Ty T -> Prop
+  inst_rel: F -> Ty T -> Ty T -> Prop
+  inst_cen: F -> Ty T -> Ty T -> Prop
+
+
+structure InstructionSet.inst {F: Type u} {T: Type v}
+  [HasLin T] [InstructionSet F T]
+  (f: F) (p: Bool) (q: Transparency) (A B: Ty T) where
+  well_typed: inst_ty f A B
+  inst_aff: (q.aff → inst_aff f A B)
+  insrt_rel: (q.rel → inst_rel f A B)
+  inst_cen: (p → inst_cen f A B)
+
+open InstructionSet
+
+inductive Term {T F: Type u} [HasLin T] [InstructionSet F T]
+  : Ctx T -> Bool -> Ty T -> Transparency -> Type u
+  | var {Γ A q} (p) (v: Ctx.var Γ ⟨q, A⟩): Term Γ p A q
+  | app {Γ} {f: F} {p A B} (Hf: inst f p q A B): Term Γ p A q -> Term Γ p B q
+  | pair {Γ Δ Ξ A B q}: Ctx.ssplit Γ Δ Ξ
+    -> Term Δ true A q
+    -> Term Ξ true B q
+    -> Term Γ true (Ty.tensor A B) q
+  | unit (p) (v: Ctx.wk Γ []) (q): Term Γ p Ty.unit q
+  | tt (p) (v: Ctx.wk Γ []) (q): Term Γ p Ty.bool q
+  | ff (p) (v: Ctx.wk Γ []) (q): Term Γ p Ty.bool q
+  | let1 {Γ Δ Ξ A B q} (p): Ctx.ssplit Γ Δ Ξ
+    -> Term Ξ true A q
+    -> Term (⟨⟨true, true⟩, A⟩::Δ) p B q
+    -> Term Γ p B q
+  | let2 {Γ Δ Ξ A B C q} (p): Ctx.ssplit Γ Δ Ξ
+    -> Term Ξ true (Ty.tensor A B) q
+    -> Term (⟨⟨true, true⟩, A⟩::⟨⟨true, true⟩, B⟩::Δ) p C q
+    -> Term Γ p C q
+
+inductive Cf {T: Type u} [HasLin T]: GCtx T -> LCtx T -> Type
   -- TODO
 
-inductive Term.subst {T} [HasLin T]: Ctx T -> Ctx T -> Type
-  | nil {Γ} (H: Ctx.wk Γ []): subst Γ []
-  | cons {Θ ΘΓ Γ Θx x}
-    (s: Ctx.ssplit Θ ΘΓ Θx)
-    (HΘΓ: subst ΘΓ Γ)
-    (HΘx: HasLin.lin Θx x.toTransparency)
-    (t: Term Θx x)
-    : subst Θ (x::Γ)
+def Block {T: Type u} [HasLin T] (Γ: Ctx T) (L: LCtx T) := Cf (GCtx.df Γ) L
+def Cfg {T: Type u} [HasLin T] (L: LCtx T) (K: LCtx T) := Cf (GCtx.cf L) K
+
+-- inductive Term.subst {T} [HasLin T]: Ctx T -> Ctx T -> Type
+--   | nil {Γ} (H: Ctx.wk Γ []): subst Γ []
+--   | cons {Θ ΘΓ Γ Θx x}
+--     (s: Ctx.ssplit Θ ΘΓ Θx)
+--     (HΘΓ: subst ΘΓ Γ)
+--     (HΘx: HasLin.lin Θx x.toTransparency)
+--     (t: Term Θx x)
+--     : subst Θ (x::Γ)
